Filrb/Internal/Invariants.lean
@@ -20,13 +20,43 @@ theorem size_nil : (.nil : Raw α).size = 0 := by
 theorem size_node : (.node l d c r : Raw α).size = l.size + r.size + 1 := by
   rfl
 
-variable [Preorder α] [Ord α] [LawfulOrd α]
 
-theorem height_le_log_size {t : Raw α} (h1 : ChildInv t) (h2 : HeightInv t) :
-    t.height ≤ 2 * Nat.log 2 t.size + 2 := by
-    induction t with
-    | nil => simp[height, size]
-    | node left data color right hleft hright => sorry
+@[simp]
+theorem height_nil : (.nil : Raw α).height = 0 := by
+  rfl
+
+@[simp]
+theorem height_node : (.node l d c r : Raw α).height = max l.height r.height + 1 := by
+  rfl
+
+theorem height_le_blackHeight' {t : Raw α} (h1 : ChildInv t) (h2 : HeightInv t) :
+    t.height ≤ 2 * t.blackHeightLeft + (if t.rootColor = .black then 0 else 1) := by
+  induction t with
+  | nil => simp
+  | node left data color right lih rih => aesop (add unsafe tactic (by omega))
+
+theorem height_le_blackHeight {t : Raw α} (h1 : ChildInv t) (h2 : HeightInv t)
+    (h : t.rootColor = .black) :
+    t.height ≤ 2 * t.blackHeightLeft := by
+  have := height_le_blackHeight' h1 h2
+  simp_all
+
+theorem blackHeight_le_size {t : Raw α} (h1 : ChildInv t) (h2 : HeightInv t) :
+    2 ^ t.blackHeightLeft ≤ t.size + 1 := by
+  induction t with
+  | nil => simp
+  | node l d c r lih rih =>
+    cases c <;> aesop (add unsafe tactic (by omega))
+
+theorem height_le_log_size {t : Raw α} (h1 : ChildInv t) (h2 : HeightInv t)
+    (h : t.rootColor = .black) :
+    t.height ≤ 2 * Nat.log 2 (t.size + 1) := by
+  calc
+    t.height ≤ 2 * t.blackHeightLeft := height_le_blackHeight h1 h2 h
+    _ ≤ 2 * Nat.log 2 (t.size + 1) := by
+      have ha2 := Nat.log_mono_right (b := 2) (blackHeight_le_size h1 h2)
+      rw [Nat.log_pow (hb := by decide)] at ha2
+      omega
 
 end Raw
 end Internal
